Update Dutch_National_Flag.thy
Added a monad version of the DNFP algortihm

Monad_Play Around/Dutch_National_Flag.thy
@@ -4,6 +4,14 @@ imports
   "~~/src/HOL/Library/State_Monad"
 
 begin
+
+text\<open>Monad definitions to encode and extract data from the monad\<close>
+definition return:: "'a \<Rightarrow> ('b, 'a) state" where "return = State_Monad.return"
+definition get:: "(nat list, nat list) state" where "get = State (\<lambda>x. (x,x))"
+definition put:: "nat list \<Rightarrow> (nat list, unit) state" where "put x = State (\<lambda>_. ((),x))"
+definition skip:: "(nat list, unit) state" where "skip = State (\<lambda>x. ((),x))"
+
+
 definition swap:: "'a list \<Rightarrow> nat \<Rightarrow> nat \<Rightarrow> 'a list" where
 "swap xs i j \<equiv> (if i < length xs \<and> j < length xs then xs[i := xs!j, j := xs!i] else xs)"
 
@@ -19,13 +27,70 @@ value\<open>swap [a,b,c,d,e] 0 4 = [e,b,c,d,a]\<close>
 text\<open>The algorithm is constant so n is originally defined as the size of the list.
       s is the list I am sorting
       low is the bound of sorted array
-      i is the current element being investigated
-      mid is the bound to for adding it two the higher or lower part of the array\<close>
-fun dnfp:: "nat \<Rightarrow> nat list \<Rightarrow> nat \<Rightarrow> nat \<Rightarrow> nat  \<Rightarrow> nat list" where
+      i is the current element being investigated\<close>
+fun dnfp:: "nat \<Rightarrow> nat list \<Rightarrow> nat \<Rightarrow> nat \<Rightarrow> nat \<Rightarrow> nat list" where
 "dnfp 0 s _ _ _ = s"|
-"dnfp n s low high i = (if high > i then (if s!i < 1 then (dnfp (n-1) (swap s i low) (Suc low) high (Suc i))
-                                else (if s!i > 1 then (dnfp (n-1) (swap s i (high-1)) low (high-1) i)
-                                  else (dnfp (n-1) s low high (Suc i)))) else s)"
+"dnfp (Suc 0) s _ _ _ = s"|
+"dnfp (Suc n) s low high i = (if high > i then (if s!i < 1 then (dnfp n (swap s i low) (Suc low) high (Suc i))
+                                else (if s!i > 1 then (dnfp n (swap s i (high-1)) low (high-1) i)
+                                  else (dnfp n s low high (Suc i))))
+                             else s)"
+
+text\<open>Is this better - with the let and (Suc high)?\<close>
+fun dnfp1:: "nat \<Rightarrow> nat list \<Rightarrow> nat \<Rightarrow> nat \<Rightarrow> nat \<Rightarrow> nat list" where
+"dnfp1 0 s _ _ _ = s"|
+"dnfp1 (Suc 0) s _ _ _ = s"|
+"dnfp1 (Suc n) s low (Suc high) i = (if (Suc high) > i then (
+                                  let (xs, l, h, j) = (if s!i < 1 then ((swap s i low), (Suc low), (Suc high), (Suc i))
+                                                 else (if s!i > 1 then ((swap s i high), low, high, i)
+                                                 else (s, low, (Suc high), (Suc i))))
+                                  in (dnfp1 n xs l h j))
+                             else s)"
+
+text\<open>A version using a state monad for storing the list/array that is being sorted\<close>
+fun dnfp_mon:: "nat \<Rightarrow> nat \<Rightarrow> nat \<Rightarrow> nat \<Rightarrow> (nat list, unit) state" where
+"dnfp_mon 0 _ _ _ = skip"|
+"dnfp_mon (Suc 0) _ _ _ = skip"|
+"dnfp_mon (Suc n) low high i = (if high > i then 
+                                do{
+                                  s \<leftarrow> get;
+                                  (if s!i < 1 then do {
+                                            s \<leftarrow> return(swap s i low);
+                                            put s;
+                                            dnfp_mon n (Suc low) high (Suc i)
+                                          }
+                                   else (if s!i > 1 then do
+                                          {
+                                            s \<leftarrow> return(swap s i (high-1)); 
+                                            put s;
+                                            dnfp_mon n low (high - 1) i
+                                          }
+                                       else dnfp_mon n low high (Suc i)))
+                                }
+                             else skip)"
+
+value \<open>snd(run_state (dnfp_mon 5 0 5 0) [0,2,2,1,2])\<close>
+value \<open>snd(run_state (dnfp_mon 9 0 9 0) [0,2,2,0,1,0,2,1,2])\<close>
+value \<open>snd(run_state (dnfp_mon 3 0 3 0) [2,1,0])\<close>
+
+value \<open>sorted(snd(run_state (dnfp_mon 5 0 5 0) [0,2,2,1,2]))\<close>
+value \<open>sorted(snd(run_state (dnfp_mon 9 0 9 0) [0,2,2,0,1,0,2,1,2]))\<close>
+value \<open>sorted(snd(run_state (dnfp_mon 3 0 3 0) [2,1,0]))\<close>
+
+
+lemma length_dnfp: "length(dnfp n xs k j k) = length xs"
+  apply(induction n)
+   apply(simp)
+    apply(simp add: swap_def length_swap)
+  apply(simp)
+  sorry
+
+lemma distinct_dnfp[simp]:
+  "distinct(dnfp n xs k j k) = distinct xs"
+  apply(induction n)
+   apply(simp)
+   apply(simp add: swap_def)
+  sorry
 
 fun dnfp_alt:: "nat list \<Rightarrow> nat list \<Rightarrow> nat \<Rightarrow> nat \<Rightarrow> nat \<Rightarrow> nat \<Rightarrow> nat list" where
 "dnfp_alt [] s _ _ _ _ = s"|
@@ -33,11 +98,9 @@ fun dnfp_alt:: "nat list \<Rightarrow> nat list \<Rightarrow> nat \<Rightarrow> 
                                       else (if s!i > mid then (dnfp_alt xs (swap s i (high-1)) low (high-1) i mid)
                                        else (dnfp_alt xs s low high (Suc i) mid))) else s)"
 
-value\<open>(dnfp_alt [0,0,2,2,1] [0,0,2,2,1] 0 5 1 1) = [0,0,1,2,2]\<close>
-value\<open>(dnfp_alt [1,0,2,0,2,0,2,1] [1,0,2,0,2,0,2,1] 0 8 1 1) = [0,0,0,1,1,2,2,2]\<close>
 
 text\<open>How do I evaluate this - where I define a variable/constant and use it in a function call\<close>
-value\<open>(\<lbrakk>xs = [0,0,2,2,1]\<rbrakk> \<Longrightarrow> (dnfp (length xs) xs 0 (length xs) 1 = [0,0,1,2,2]))\<close>
+value\<open>(xs = [0,0,2,2,1] \<Longrightarrow> (dnfp (length xs) xs 0 (length xs) 1 = [0,0,1,2,2]))\<close>
 
 
 value\<open>(dnfp 5 [0,0,2,2,1] 0 5 1) = [0,0,1,2,2]\<close>
@@ -47,6 +110,12 @@ value\<open>sorted(dnfp 7 [1,0,2,0,2,2,1] 0 7 1 )\<close>
 value\<open>sorted(dnfp 8 [1,0,2,0,2,2,1,0] 0 8 1 )\<close>
 value\<open>(dnfp 8 [1,0,2,0,2,2,1,0] 0 8 1)\<close>
 
+value\<open>(dnfp1 5 [0,0,2,2,1] 0 5 1) = [0,0,1,2,2]\<close>
+value\<open>(dnfp1 8 [1,0,2,0,2,0,2,1] 0 8 1) = [0,0,0,1,1,2,2,2]\<close>
+value\<open>sorted(dnfp1 8 [1,0,2,0,2,0,2,1] 0 8 1)\<close>
+value\<open>sorted(dnfp1 7 [1,0,2,0,2,2,1] 0 7 1 )\<close>
+value\<open>sorted(dnfp1 8 [1,0,2,0,2,2,1,0] 0 8 1 )\<close>
+value\<open>(dnfp1 8 [1,0,2,0,2,2,1,0] 0 8 1)\<close>
 
 
 end
